---
layout: post
title: 1442. Count Triplets That Can Form Two Arrays of Equal XOR
gh-repo: yukinj
gh-badge: [star, fork, follow]
tags: [Array,Bit Manipulation,Math]
comments: true
---

```python
class Solution:
    def countTriplets(self, A: List[int]) -> int:
        """
        
       tc O(N^2)  sc O(1) prefix XOR 
                      assuming a = A[i] ^ A[i+1] ^...A[j-1], b = A[j]^A[j+1]^...A[k] 
        main idea3: - a == b => a^a == a^b => A[i]^A[i+1]^...A[k] == 0  => prefix[k+1] = prefix[i]
                    - find out how many pair(i,k) of prefix value are equal 
                    1. calculate prefix array
                    2. brute force count the pair (i,k)  =>  since  i < j <=k  => res += j-i 
        
        
        """
        res,n = 0,len(A)
        for i in range(n):
            xor = A[i]
            for j in range(i+1,n):
                xor ^= A[j]
                if xor == 0:
                    res += j-i
        return res 

```


O(N)
```python
class Solution:
    def countTriplets(self, A: List[int]) -> int:
        """
       tc O(N)  sc O(N) prefix XOR 
       
       => find sum of index distance with A[i] = A[j]
       - count the frequency and total value at the same time 
        main idea: given array A[0],A[1],A[2],...A[n-1], 
                    assuming at index j, if xor(A[0:i]) inclusive has appeared before, then sor(A[j+1:i]) = 0
                    if xor(A[i:j]) = 0, then A[i:j] will add (j-i-1) to the answer 

                    assuming xor(A[0:i]) = x, and x hass occurred 3 time before at index i1,i2,i3
                    answer for i will be = (i-i1-1)+(i-i2-1)+(i-i3-1) => f*i-(i1+i2+i3) - f = f*(i-1) -(i1+i2+i3);  where f : number of times x has occurred previously; (i1+i2+i3):  sum of index where x has occurred   

        """
        A.insert(0,0)
        res,n = 0,len(A)
        pxor = [0] *n
        for i in range(1,n):
            pxor[i] = pxor[i-1]^A[i]

        cnt,total = defaultdict(int),defaultdict(int)
        for j in range(n):
            res += cnt[pxor[j]]*(j-1)-total[pxor[j]]
            cnt[pxor[j]] += 1 # cnt # same prefix xor
            total[pxor[j]] += j # sum of index when prefix[j] == prefix[i]
        
        return res

```
